examples/ecc: update exponentiation example

src/Rupicola/Examples/ECC/Exponentiation.v
@@ -1,4 +1,5 @@
 Require Import Rupicola.Lib.Api.
+Require Import Rupicola.Lib.Loops.
 Require Import Rupicola.Examples.ECC.Field.
 Local Open Scope Z_scope.
 
@@ -26,9 +27,9 @@ Section S.
     Local Infix "^" := (fun x y => (x ^ y) mod M).
 
     Definition exp_by_squaring_6 (x : Z) : Z :=
-      let/d x2 := x ^ 2 in
-      let/d x3 := x2 * x in
-      let/d x6 := x3 ^ 2 in
+      let/d x2 := (x mod M) ^ 2 in
+      let/d x3 := (x2 mod M) * (x mod M) in
+      let/d x6 := (x3 mod M) ^ 2 in
       x6.
 
     Lemma mod_equal :
@@ -74,10 +75,10 @@ Section S.
       match n with
       | xH => x mod M
       | xO xH => x^2 mod M
-      | xI xH => let/n res := x^2 in x * res
-      | xO n' => let/n res := exp_by_squaring x n' in res^2
-      | xI n' => let/n res := exp_by_squaring x n' in
-                 let/n res := res^2 in
+      | xI xH => let/n res := x^2 mod M in x * res
+      | xO n' => let/n res := exp_by_squaring x n' mod M in res^2
+      | xI n' => let/n res := exp_by_squaring x n' mod M in
+                 let/n res := res^2 mod M in
                  x * res
       end.
 
@@ -132,7 +133,6 @@ Section S.
     Qed.
     Print rewritten.
 
-    (*
     Lemma exp_by_squaring_correct :
       M <> 0 -> forall n x, exp_by_squaring x n = x ^ (Zpos n).
     Proof.
@@ -140,23 +140,46 @@ Section S.
       - rewrite IHn.
         rewrite mod_exp by assumption.
         rewrite Z.mul_mod_idemp_r by assumption.
-        apply mod_equal.
-        rewrite Pos2Z.pos_xI.
-        rewrite Z.pow_add_r by lia.
-        rewrite <- Z.pow_mul_r by lia.
-        rewrite Z.mul_comm with (n := 2).
-        lia.
+        destruct n eqn : H'.
+        + rewrite <- H'.
+          rewrite Pos2Z.pos_xI.
+          rewrite Z.pow_add_r; try easy.
+          rewrite Z.pow_1_r.
+          rewrite Z.pow_2_r.
+          Z.push_pull_mod.
+          rewrite Z.pow_twice_r.
+          rewrite Z.mul_comm.
+          reflexivity.
+        + rewrite <- H'. change (Z.pos ?n~1) with (2 * Z.pos n + 1)%Z.
+          rewrite Z.pow_add_r; try easy.
+          rewrite Z.pow_1_r.
+          rewrite Z.pow_2_r.
+          Z.push_pull_mod.
+          rewrite Z.pow_twice_r.
+          rewrite Z.mul_comm.
+          reflexivity.
+        + Z.push_pull_mod.
+          reflexivity.
       - rewrite IHn.
         rewrite mod_exp by assumption.
-        apply mod_equal.
-        symmetry. rewrite Pos2Z.pos_xO.
-        rewrite <- Z.pow_mul_r by lia.
-        rewrite Z.mul_comm with (n := 2).
-        lia.
+        destruct n eqn : H'; try reflexivity.
+        + rewrite <- H'.
+          rewrite Pos2Z.pos_xO.
+          rewrite Z.pow_2_r.
+          change (Z.pos ?n~0) with (2 * Z.pos n)%Z.
+          rewrite Z.pow_twice_r.
+          Z.push_pull_mod.
+          reflexivity.
+        + rewrite <- H'. change (Z.pos ?n~0) with (2 * Z.pos n)%Z.
+          rewrite Z.pow_mul_r; try easy.
+          rewrite Z.pow_twice_r.
+          rewrite Z.pow_1_r.
+          rewrite Z.pow_2_r.
+          Z.push_pull_mod.
+          reflexivity.
       - rewrite Z.pow_1_r.
         reflexivity.
     Qed.
-    *)
   End Gallina.
 
   Section Bedrock.
@@ -208,14 +231,14 @@ Section S.
              | [ H : context[postcondition_func_norets] |- _ ] => destruct H
              end.
 
-
+(*
     Lemma exp_6_correct : program_logic_goal_for_function! exp_6.
     Proof.
       repeat straightline.
       intros; exists [x_ptr; sq_ptr]; split.
       - subst l. tac.
       - subst l. tac.
-    Admitted.
+    Admitted.*)
 
     Definition exp_result x_ptr q_ptr xq_val : list word -> Semantics.mem -> Prop :=
       fun _ => Lift1Prop.ex1 (fun x => Lift1Prop.ex1 (fun q =>
@@ -224,9 +247,9 @@ Section S.
                                                           (Bignum x_ptr x * Bignum q_ptr q)))%sep)).
 
     Definition exp_by_squaring_6' (x : Z) : (Z * Z) :=
-      let/n out := x ^ 2 mod M in
-      let/n out := out * x mod M in
-      let/n out := out ^ 2 mod M in
+      let/n out := (x mod M) ^ 2 mod M in
+      let/n out := out * (x mod M) mod M in
+      let/n out := out  ^ 2 mod M in
       (x, out).
 
     Lemma Lift1Prop_impl1_ex :
@@ -259,22 +282,22 @@ Section S.
     Qed.
 
     Ltac field_cleanup :=
-      Z.push_pull_mod; pull_mod;
+      (* Z.push_pull_mod; pull_mod; *)
       match goal with
       | [ H: _ mod _ = ?v |- _ ] => is_var v; rewrite <- H
       | _ => idtac
       end.
 
     Ltac compile_custom ::=
-      progress (field_cleanup;
+      progress ( field_cleanup;
                 try (try simple eapply compile_dlet_as_nlet_eq;
                      try simple eapply compile_nlet_as_nlet_eq;
                      first [ simple eapply compile_square
                            | simple eapply compile_mul]));
       (intros; unfold Placeholder in *).  (* FIXME get rid of placeholders? *)
 
-    Hint Unfold exp_result : compiler_cleanup.
-
+       Hint Unfold exp_result : compiler_cleanup.
+       
     Derive exp_body SuchThat
            (let exp6 := ("exp6", (["x"; "out"], [], exp_body)) in
             program_logic_goal_for exp6
@@ -294,15 +317,18 @@ Section S.
                                               R tr)))
            As exp_body_correct.
     Proof.
-      compile.
-      lift_eexists; sepsimpl; eauto || ecancel_assumption.
+      compile_setup.
+      repeat compile_step.
+      lift_eexists; sepsimpl. eauto || ecancel_assumption.
+      eapply Heq1.
+      ecancel_assumption.
     Qed.
 
     Definition exp_by_squaring_9' (x : Z) : (Z * Z) :=
-      let/n out := x ^ 2 mod M in
+      let/n out := (x mod M) ^ 2 mod M in
       let/n out := out ^ 2 mod M in
       let/n out := out ^ 2 mod M in
-      let/n out := x * out mod M in
+      let/n out := x mod M * out mod M in
       (x, out).
 
     Derive exp9_body SuchThat
@@ -325,16 +351,12 @@ Section S.
            As exp9_body_correct.
     Proof.
       compile.
-      lift_eexists; sepsimpl; eauto || ecancel_assumption.
+      lift_eexists; sepsimpl; eauto || ecancel_assumption. 
     Qed.
 
-    (* Lemma Zmult_mod_idemp_r_inplace : *)
-    (*   forall a b n : Z, *)
-    (*     (b * inplace (a mod n)) mod n = (b * inplace(a)) mod n. *)
-    (*   unfold inplace. *)
-    (*   apply Zmult_mod_idemp_r. *)
-    (* Qed. *)
+    Compute exp9_body.
 
+(*
     Derive exp_11_body SuchThat
            (let exp11 := ("exp11", (["x"; "res"], [], exp_11_body)) in
             program_logic_goal_for exp11
@@ -357,7 +379,7 @@ Section S.
     Proof.
       compile.
       lift_eexists; sepsimpl; eauto || ecancel_assumption.
-    Qed.
+    Qed.*)
 
     Fixpoint run_length_encoding (n : positive) : list (bool * nat) :=
       match n with
@@ -378,7 +400,7 @@ Section S.
 
     Fixpoint loop {A} (x : A) (k : nat) (f : A -> A) : A :=
       match k with
-      | 0%nat => f x
+      | 0%nat => x
       | S k' => f (loop x k' f)
       end.
 
@@ -394,21 +416,21 @@ Section S.
         1
       (* can add more cases for small k to be faster *)
       | (true, 0%nat) :: t =>
-        let/n res := exp_from_encoding x t in
+        let/n res := exp_from_encoding x t mod M in
         let/n res := res^2 mod M in
         let/n res := x * res mod M in
         res
       | (true, k) :: t =>
-        let/n res := exp_from_encoding x t in
-        let/n res := loop res k (exp_square_and_multiply x) in
+        let/n res := exp_from_encoding x t mod M in
+        let/n res := loop res (S k) (exp_square_and_multiply x) in
         res
       | (false, 0%nat) :: t =>
-        let/n res := exp_from_encoding x t in
+        let/n res := exp_from_encoding x t mod M in
         let/n res := res^2 mod M in
         res
       | (false, k) :: t =>
-        let/n res := exp_from_encoding x t in
-        let/n res := loop res k (exp_square) in
+        let/n res := exp_from_encoding x t mod M in
+        let/n res := loop res (S k) (exp_square) in
         res
       end.
 
@@ -417,45 +439,312 @@ Section S.
 
     Compute run_length_encoding 4.
 
-    (*
-    Lemma exp_by_squaring_encoded_correct :
+    Lemma run_length_encoding_nonempty:
+      forall n, run_length_encoding n <> [].
+    Proof.
+      destruct n eqn : H'; simpl.
+      + destruct (run_length_encoding p).
+        { inversion 1. }
+        destruct p0; destruct b; inversion 1.
+      + destruct (run_length_encoding p).
+        { inversion 1. }
+        destruct p0; destruct b; inversion 1.
+      + inversion 1.
+    Qed.
+
+    Lemma exp_by_squaring_encoded_correct : 
       M <> 0 -> forall n x, exp_by_squaring_encoded x n = x ^ (Zpos n) mod M.
     Proof.
       intros. rewrite <- exp_by_squaring_correct; eauto.
       unfold exp_by_squaring_encoded; induction n; simpl.
       - cbn -[loop].
-        destruct (run_length_encoding n).
-        + rewrite <- IHn. eauto.
+        destruct (run_length_encoding n) eqn : Heq.
+        + apply run_length_encoding_nonempty in Heq.
+          inversion Heq.
         + destruct p. destruct b.
           { rewrite <- IHn.
-          cbn. replace (n0 + 1)%nat with (S n0).
-          { unfold nlet; destruct n0.
+          cbn. replace (n0 + 1)%nat with (S n0) by lia.
+          unfold nlet; destruct n0.
             { cbn.
+              destruct n eqn : H'.
+              { repeat eapply mod_equal.
+                unfold exp_square_and_multiply.
+                rewrite <- Z.mul_comm.
+                f_equal.
+                rewrite ! Z.pow_2_r.
+                Z.push_pull_mod.
+                f_equal.
+                ring.
+              }
+              { repeat eapply mod_equal.
+                unfold exp_square_and_multiply.
+                rewrite <- Z.mul_comm.
+                f_equal.
+                rewrite ! Z.pow_2_r.
+                Z.push_pull_mod.
+                f_equal.
+                ring.
+              }
+              {
+              unfold run_length_encoding in Heq.
+              inversion Heq.
               repeat eapply mod_equal.
+              unfold exp_square_and_multiply.
+              unfold exp_from_encoding.
               rewrite <- Z.mul_comm.
               f_equal.
-              eapply mod_equal.
-              set ((exp_from_encoding x l)) as exl.
-              ring_simplify.
-              rewrite <- Z.mul_comm. reflexivity.
+              rewrite ! Z.pow_2_r.
+              Z.push_pull_mod.
+              f_equal.
+              ring.
+              }
             }
-            eapply mod_equal.
-            eapply Z.mul_comm.
+            cbn.
+            destruct n eqn : H'.
+            { repeat eapply mod_equal.
+              Z.push_pull_mod.
+                unfold exp_square_and_multiply.
+                rewrite <- Z.mul_comm.
+                f_equal.
+            }
+            { repeat eapply mod_equal.
+              Z.push_pull_mod.
+                unfold exp_square_and_multiply.
+                rewrite <- Z.mul_comm.
+                f_equal.
+            }
+            
+              {
+              unfold run_length_encoding in Heq.
+              inversion Heq.
+              }
           }
-          { symmetry. eapply Nat.add_1_r. }
+          rewrite <- IHn.
+          cbn.
+          unfold nlet.
+          destruct n0; destruct n eqn : H'; try reflexivity.
+          { unfold run_length_encoding in Heq.
+            Z.push_pull_mod.
+            inversion Heq.
           }
-        rewrite <- IHn. cbn. unfold nlet. eauto.
+          unfold run_length_encoding in Heq.
+          inversion Heq.
       - rewrite <- IHn.
+        cbn. 
+        destruct n eqn : H'.
+        { destruct (run_length_encoding p~1) as [|[[|] n0] t]; try reflexivity.
+          simpl.
+          replace (n0 + 1)%nat with (S n0) by lia.
+          unfold nlet.
+          cbn.
+          unfold exp_square.
+          destruct n0.
+          { unfold loop.
+            set (exp_from_encoding x t mod M) as ext.
+            rewrite <- Z.pow_mod.
+            Z.push_pull_mod.
+            f_equal.
+          }
+          set (exp_from_encoding x t mod M) as ext.
+          rewrite Z.mul_1_r.
+          set (loop ext (S n0) (fun x' : Z => x' ^ 2 mod M) mod M) as lext.
+          f_equal.
+          Z.push_pull_mod.
+          ring.
+        }
+        { destruct (run_length_encoding p~0) as [|[[|] n0] t]; try reflexivity.
+          simpl.
+          replace (n0 + 1)% nat with (S n0) by lia.
+          unfold nlet.
+          cbn.
+          unfold exp_square.
+          destruct n0.
+          { unfold loop.
+            set (exp_from_encoding x t mod M) as ext.
+            rewrite Z.mul_1_r.
+            rewrite <- Z.pow_mod.
+            Z.push_pull_mod.
+            f_equal.
+            ring.
+          }
+          set (exp_from_encoding x t mod M) as ext.
+          rewrite Z.mul_1_r.
+          set (loop ext (S n0) (fun x' : Z => x' ^ 2 mod M)) as lext.
+          Z.push_pull_mod.
+          rewrite <- Z.pow_mod.
+          f_equal.
+          ring.
+        }
+        inversion IHn.
+        unfold nlet in H1.
+        unfold run_length_encoding.
+        unfold exp_from_encoding.
+        unfold nlet.
+        rewrite Z.pow_2_r.
+        rewrite <- Z.pow_mod.
+        Z.push_pull_mod.
+        f_equal.
+        ring.
+      - unfold nlet.
         cbn.
-        destruct (run_length_encoding n) as [|[[|] n0] t]; eauto.
-        rewrite Nat.add_comm.
-        destruct n0; eauto.
-      - unfold nlet; cbn.
-        rewrite Zmult_mod_idemp_r.
-        eapply mod_equal.
-        apply Z.mul_1_r.
+        Z.push_pull_mod.
+        rewrite Z.mul_1_r.
+        reflexivity.
     Qed.
-    *)
+
+    Definition exp_by_squaring_encoded_6' (x : Z) : (Z * Z) :=
+      let/n out := x ^ 2 mod M in
+      let/n out := loop out 7 (fun out => let/n out := exp_square out in out) in
+      (x, out).
+
+    Lemma loop_equals':
+      forall {A} f (x : A) k,
+        (ExitToken.new, loop x k f) =
+      (ranged_for' 0 (Z.of_nat k)
+       (fun (tok : ExitToken.t) (idx : Z) (acc : A) _ =>
+          (tok, f acc)) x).
+    Proof.
+      induction k.
+      - simpl.
+        unfold ranged_for'.
+        rewrite ranged_for_break_exit; try reflexivity.
+        lia.
+      - cbn -[Z.of_nat].
+        replace (Z.of_nat (S k)) with (Z.of_nat k + 1) by lia.
+        erewrite ranged_for'_unfold_r_nstop; try lia; try easy.
+        all: rewrite <- IHk; reflexivity.
+    Qed.
+    
+        
+    Lemma loop_equals :
+      forall {A} f (x : A) k,
+        Z.of_nat k < 2 ^ Semantics.width ->
+        loop x k f =
+        let/n from := 0 in
+        let/n to := word.of_Z (Z.of_nat k) in
+        ranged_for_u (word.of_Z from) to
+                     (fun t _ acc _ =>
+                        let/n out := f acc in (t, out)) x.
+    Proof.
+      intros.
+      unfold nlet.
+      unfold ranged_for_u in *.
+      unfold ranged_for_w in *.
+      unfold ranged_for in *.
+      unfold w_body.
+      pose proof Nat2Z.is_nonneg k.
+      pose proof Nat2Z.is_nonneg (S k).
+      repeat rewrite word.unsigned_of_Z_0.
+      repeat rewrite word.unsigned_of_Z.
+      repeat rewrite word.wrap_small by lia.
+      rewrite <- loop_equals'.
+      reflexivity.
+    Qed.
+
+    Lemma Znum_to_Bignum :
+      forall R mem x_ptr x, (Znum x_ptr x * R)%sep mem ->
+                            exists b : bignum, (x = eval b mod M) /\
+                                               (Bignum x_ptr b * R)%sep mem.
+      intros.
+      unfold Znum in *.
+      destruct H as (? & ? & ? & ? & ?).
+      destruct H0 as (? & ? & ?).
+      exists x2.
+      split.
+      - apply H0.
+      - unfold sep. exists x0. exists x1. split.
+        + apply H.
+        + split.
+          apply H2.
+          apply H1.
+      Qed.
+
+
+  
+   Definition exp_result' x_ptr q_ptr xq_val : list word -> Semantics.mem -> Prop :=
+     fun _ => (Znum x_ptr (fst xq_val) * Znum q_ptr (snd xq_val))%sep.
+
+   Hint Unfold exp_result' : compiler_cleanup.
+   Hint Unfold exp_square : compiler_cleanup.
+
+   Hint Extern 1 => simple eapply compile_Z_square; shelve : compiler.
+
+       (*
+   Ltac compile_copy :=
+      match goal with
+      | [ H: (Znum ?ptr ?v * ?R)%sep ?m |- ?l ] =>
+        match l with
+        | context [map.put _ ?x ptr] =>
+          match l with
+            | context [let/n _ as x eq:_ := v in _] =>
+            apply compile_copy_pointer with (var := x) (x_ptr0 := ptr) (Data := Znum) (R0 := R)
+          end
+        end
+      end.*)
+
+   Ltac compile_try_copy_pointer :=
+     lazymatch goal with
+     | [ H : ?pred ?m |- WeakestPrecondition.cmd _ _ _ ?m ?l (_ ?term) ] =>
+       match term with
+       | nlet_eq [?var_] ?v _ =>
+         match l with
+         | context [map.put _ var_ ?ptr] =>
+           match pred with
+           | context [?Data_ ptr v] =>
+             simple eapply compile_copy_pointer with (var := var_) (x_ptr0 := ptr) (Data := Data_)
+           end
+         end
+       end
+     end.
+
+   Ltac compile_custom ::=
+     progress ( field_cleanup;
+                try rewrite loop_equals;
+                try (try simple eapply compile_dlet_as_nlet_eq;
+                     try simple eapply compile_nlet_as_nlet_eq;
+                     first [ simple eapply compile_square
+                           | simple eapply compile_mul
+                           | compile_try_copy_pointer]));
+     intros.
+
+   Lemma clean_width :
+     forall x, x < 2 ^ 32 -> x < 2 ^ Semantics.width.
+   Proof.
+     intros; destruct Semantics.width_cases as [ -> | -> ]; lia.
+   Qed.
+
+   Hint Extern 1 => simple eapply clean_width; reflexivity : compiler_cleanup.
+     
+    Derive exp_body' SuchThat
+           (let exp6_encoded := ("exp6", (["x"; "out"], [], exp_body')) in
+            program_logic_goal_for exp6_encoded
+                                   (forall functions,
+                                       spec_of_Z_UnOp un_square functions ->
+                                       spec_of_Z_BinOp bin_mul functions ->
+                                       forall x_ptr x sq_ptr sq_init tr R mem,
+                                         (*bounded_by tight_bounds x ->*)
+                                         (*bounded_by tight_bounds sq_init ->*)
+                                         ((Znum x_ptr x * Znum sq_ptr sq_init * R)%sep mem) ->
+                                         WeakestPrecondition.call
+                                           (exp6_encoded :: functions)
+                                           "exp6"
+                                           tr mem [x_ptr; sq_ptr]
+                                           (postcondition_func_norets
+                                              (exp_result' x_ptr sq_ptr (exp_by_squaring_encoded_6' x))
+                                              R tr)))
+           As exp_body_correct'.
+    compile.
+    simple apply compile_nlet_as_nlet_eq.
+    
+    eapply compile_ranged_for_u with (loop_pred := (fun idx z tr' mem' locals' =>
+         tr' = tr /\
+         locals' = map.put
+                 (map.put (map.put (map.put map.empty "x" x_ptr) "out" sq_ptr) "from"
+                    idx) "to" v1 /\
+         (Znum sq_ptr z ⋆ (Znum x_ptr x ⋆ R)) mem')); repeat compile_step.
+            
+    Qed.
+        
   End Bedrock.
 
 End S.
